WIP to plug the correctness of the initialization into the main theorem

coq/LLVMGen/Correctness.v
@@ -2384,6 +2384,7 @@ Proof.
   auto.
 Qed.
 
+From Vellvm Require Import AstLib.
 (* Lemma bisim_full_partial_subrelation: forall σ helix_state llvm_state, *)
 (*     let '(mem_helix, v_helix) := helix_state in *)
 (*     let '(m, ((ρ,_), (g, v))) := llvm_state in *)
@@ -2397,6 +2398,33 @@ Qed.
 (*   auto. *)
 (* Qed. *)
 
+(* YZ TODO move  *)
+
+  Definition opt_first {T: Type} (o1 o2: option T): option T :=
+    match o1 with | Some x => Some x | None => o2 end.
+
+  Definition modul_app {T X} (m1 m2: modul T X): modul T X :=
+    let (name1, target1, layout1, tdefs1, globs1, decls1, defs1) := m1 in
+    let (name2, target2, layout2, tdefs2, globs2, decls2, defs2) := m2 in
+    {|
+      m_name := opt_first name1 name2;
+      m_target := opt_first target1 target2;
+      m_datalayout := opt_first layout1 layout2;
+      m_type_defs := tdefs1 ++ tdefs2;
+      m_globals := globs1 ++ globs2;
+      m_declarations := decls1 ++ decls2;
+      m_definitions := defs1 ++ defs2
+    |}.
+
+  Lemma modul_of_toplevel_entities_app:
+    forall {T X} tle1 tle2, 
+    @modul_of_toplevel_entities T X (tle1 ++ tle2) ≡ modul_app (modul_of_toplevel_entities T tle1) (modul_of_toplevel_entities T tle2).
+  Proof.
+    induction tle1 as [| tle tle1 IH]; intros; cbn; [reflexivity |].
+    { unfold modul_of_toplevel_entities.
+      f_equal; try reflexivity.
+  Admitted.
+
 (* Top-level compiler correctness lemma  *)
 Theorem compiler_correct:
   forall (p:FSHCOLProgram)
@@ -2406,6 +2434,48 @@ Theorem compiler_correct:
     eutt (bisim_final []) (semantics_FSHCOL p data) (semantics_llvm pll).
 Proof.
   intros p data pll H.
+  unfold compile_w_main, compile in H.
+  destruct p.
+  cbn in *.
+  break_match_hyp; try inv_sum.
+  break_let; cbn in *.
+  break_match_hyp; try inv_sum.
+  unfold ErrorWithState.evalErrS in *.
+  break_match_hyp; try inv_sum.
+  break_match_hyp; cbn in *; repeat try inv_sum.
+  break_let; cbn in *; inv_sum.
+  repeat (break_match_hyp || break_let); try inv_sum.
+
+  eutt_hide_left.
+  repeat rewrite app_assoc.
+  repeat rewrite <- app_assoc.
+  match goal with
+    |- context[_ :: ?x ++ ?y ++ ?z ++ ?t] => remember x as f1; remember y as f2; remember t as f3; remember z as f4
+  end.
+
+  (* unfold semantics_llvm, semantics_llvm_mcfg, model_to_L3, denote_vellvm_init, denote_vellvm. *)
+  (* unfold lift_sem_to_mcfg. *)
+  (* break_match_goal. *)
+  (*     destruct tle2 eqn:EQ; cbn. *)
+  (*     reflexivity. *)
+  (*   m (modul_of_toplevel_entities T tle2); cbn. *)
+  (*   unfold modul_app; cbn. *)
+
+
+(* (AstLib.modul_of_toplevel_entities typ (TLE_Comment "Global variables" :: f1 ++ f2 ++ f4 ++ f3)) *)
+
+(*   2:{ *)
+(*     Opaque map_option. *)
+(*     subst. *)
+(*     cbn in *. *)
+    
+(*     { *)
+(*   } *)
+
+
+  (* cbn. *)
+
+  (* setoid_rewrite bind_bind.  interp_to_L3_bind. *)
   (* This no longer follows from [compiler_correct_aux]. It will
      at pen-ultimate step when the [main] does [return] on a memory
      block.
@@ -2416,5 +2486,5 @@ Proof.
        tauto.
        tauto.
        tauto.
-   *)
+   *)  
 Admitted.
